compiler/src/compiler/UpperPipeline.v
@@ -19,32 +19,19 @@ Require Import compiler.RegAlloc.
 Section WithWordAndMem.
   Context {width: Z} {BW: Bitwidth width} {word: Interface.word width} {mem : map.map word byte}.
 
-  Record Lang: Type := {
-    Var: Type;
-    Cmd: Type;
-    Locals : map.map Var word;
-    Env : map.map string (list Var * list Var * Cmd);
-    Exec: Env -> Cmd -> trace -> mem -> Locals -> MetricLog ->
-          (trace -> mem -> Locals -> MetricLog -> Prop) -> Prop
-  }.
+  Definition CallSpec(FunEnv: Type): Type :=
+    FunEnv -> string -> trace -> mem -> list word -> MetricLog ->
+    (trace -> mem -> list word -> Prop) -> Prop.
 
-  Definition phase_correct{L1 L2: Lang}(compile: L1.(Env) -> option L2.(Env)): Prop :=
-    forall functions1 functions2 f_entry_name argnames1 retnames1 fbody1,
+  Definition phase_correct{Func1 Func2: Type}
+             {env1: map.map string Func1}{env2: map.map string Func2}
+             (Call1: CallSpec env1)(Call2: CallSpec env2)
+             (compile: env1 -> option env2): Prop :=
+    forall functions1 functions2 fname,
       compile functions1 = Some functions2 ->
-      map.get functions1 f_entry_name = Some (argnames1, retnames1, fbody1) ->
-      exists argnames2 retnames2 fbody2,
-        map.get functions2 f_entry_name = Some (argnames2, retnames2, fbody2) /\
-        (* These length equalities also follow from the map.of_list_zip = Some and from the
-           map.getmany_of_list = Some below, but that's under a L1.(Exec) assumption that we don't always have *)
-        List.length argnames1 = List.length argnames2 /\
-        List.length retnames1 = List.length retnames2 /\
-        forall argvals t m l1 mc post,
-          map.of_list_zip argnames1 argvals = Some l1 ->
-          L1.(Exec) functions1 fbody1 t m l1 mc (fun t' m' l1' mc' =>
-            exists retvals, map.getmany_of_list l1' retnames1 = Some retvals /\ post t' m' retvals) ->
-          exists l2, map.of_list_zip argnames2 argvals = Some l2 /\
-            L2.(Exec) functions2 fbody2 t m l2 mc (fun t' m' l2' mc' =>
-              exists retvals, map.getmany_of_list l2' retnames2 = Some retvals /\ post t' m' retvals).
+      forall argvals t m mc post,
+        Call1 functions1 fname t m argvals mc post ->
+        Call2 functions2 fname t m argvals mc post.
 
   Definition compose_phases{A B C: Type}(phase1: A -> option B)(phase2: B -> option C)(a: A) :=
     match phase1 a with
@@ -52,20 +39,19 @@ Section WithWordAndMem.
     | None => None
     end.
 
-  Lemma compose_phases_correct{L1 L2 L3: Lang}
-        (compile12: L1.(Env) -> option L2.(Env))
-        (compile23: L2.(Env) -> option L3.(Env)):
-    phase_correct compile12 -> phase_correct compile23 -> phase_correct (compose_phases compile12 compile23).
+  Lemma compose_phases_correct{Func1 Func2 Func3: Type}
+        {env1: map.map string Func1}{env2: map.map string Func2}{env3: map.map string Func3}
+        (Call1: CallSpec env1)(Call2: CallSpec env2)(Call3: CallSpec env3)
+        (compile12: env1 -> option env2)
+        (compile23: env2 -> option env3):
+    phase_correct Call1 Call2 compile12 ->
+    phase_correct Call2 Call3 compile23 ->
+    phase_correct Call1 Call3 (compose_phases compile12 compile23).
   Proof.
-    unfold phase_correct, compose_phases. intros C12 C23. intros *. intros ? G1. simp.
-    specialize C12 with (1 := E) (2 := G1). simp.
-    specialize C23 with (1 := H) (2 := C12p0). simp.
-    eexists _, _, _. split. 1: eassumption.
-    ssplit; try congruence.
-    intros *. intros OL1 Ex1.
-    specialize C12p3 with (1 := OL1) (2 := Ex1). simp.
-    specialize C23p3 with (1 := C12p3p0) (2 := C12p3p1).
-    exact C23p3.
+    unfold phase_correct, compose_phases. intros C12 C23. intros. simp.
+    specialize C12 with (1 := E) (2 := H0).
+    specialize C23 with (1 := H) (2 := C12).
+    exact C23.
   Qed.
 
   Section WithMoreParams.
@@ -79,43 +65,40 @@ Section WithWordAndMem.
 
     Context {ext_spec_ok : Semantics.ext_spec.ok ext_spec}.
 
-    Definition SrcLang := {|
-      Var := string;
-      Cmd := Syntax.cmd;
-      Env := string_keyed_map (list string * list string * Syntax.cmd);
-      Exec := Semantics.exec
-    |}.
+    Definition SrcLang: CallSpec (string_keyed_map (list string * list string * Syntax.cmd)) :=
+      fun e f t m argvals mc post =>
+        exists argnames retnames fbody,
+          map.get e f = Some (argnames, retnames, fbody) /\
+          forall l, map.of_list_zip argnames argvals = Some l ->
+                    Semantics.exec e fbody t m l mc (fun t' m' l' mc' =>
+                      exists retvals, map.getmany_of_list l' retnames = Some retvals /\
+                                      post t' m' retvals).
 
-    Definition FlatLangStr := {|
-      Var := string;
-      Cmd := FlatImp.stmt string;
-      Env := string_keyed_map (list string * list string * FlatImp.stmt string);
-      Exec := FlatImp.exec
-    |}.
+    Definition FlatLang(Var: Type){locals: map.map Var word}:
+      CallSpec (string_keyed_map (list Var * list Var * FlatImp.stmt Var)) :=
+      fun e f t m argvals mc post =>
+        exists argnames retnames fbody,
+          map.get e f = Some (argnames, retnames, fbody) /\
+          forall l, map.of_list_zip argnames argvals = Some l ->
+                    FlatImp.exec e fbody t m l mc (fun t' m' l' mc' =>
+                      exists retvals, map.getmany_of_list l' retnames = Some retvals /\
+                                      post t' m' retvals).
 
-    Definition FlatLangZ := {|
-      Var := Z;
-      Cmd := FlatImp.stmt Z;
-      Locals := Zlocals;
-      Env := string_keyed_map (list Z * list Z * FlatImp.stmt Z);
-      Exec := FlatImp.exec
-    |}.
-
-    Lemma flattening_correct: @phase_correct SrcLang FlatLangStr flatten_functions.
+    Lemma flattening_correct: phase_correct SrcLang (FlatLang string) flatten_functions.
     Proof.
-      unfold phase_correct. intros.
+      unfold phase_correct, SrcLang, FlatLang. intros. simp.
 
-      pose proof H0 as GF.
+      pose proof H as GF.
       unfold flatten_functions in GF.
       eapply map.map_all_values_fw in GF. 5: eassumption. 2-4: typeclasses eauto.
       unfold flatten_function in GF. simp.
 
       eexists _, _, _. split. 1: eassumption.
-      intros. ssplit; try reflexivity. eexists. split. 1: eassumption.
+      intros.
       eapply FlatImp.exec.weaken.
-      - eapply flattenStmt_correct_aux.
+      - eapply flattenStmt_correct_aux with (mcH := mc).
         + eassumption.
-        + eassumption.
+        + eauto.
         + reflexivity.
         + match goal with
           | |- ?p = _ => rewrite (surjective_pairing p)
@@ -123,9 +106,9 @@ Section WithWordAndMem.
           reflexivity.
         + intros x k A. assumption.
         + unfold map.undef_on, map.agree_on. cbn. intros k A.
-          rewrite map.get_empty. destr (map.get l1 k). 2: assumption. exfalso.
-          unfold map.of_list_zip in H1.
-          edestruct (map.putmany_of_list_zip_find_index _ _ _ _ _ _ H1 E) as [G | G]. 2: {
+          rewrite map.get_empty. destr (map.get l k). 2: reflexivity. exfalso.
+          unfold map.of_list_zip in H0.
+          edestruct (map.putmany_of_list_zip_find_index _ _ _ _ _ _ H0 E) as [G | G]. 2: {
             rewrite map.get_empty in G. discriminate.
           }
           destruct G as (i & G1 & G2).
@@ -136,9 +119,9 @@ Section WithWordAndMem.
       - simpl. intros. simp. eauto using map.getmany_of_list_extends.
     Qed.
 
-    Lemma regalloc_correct: @phase_correct FlatLangStr FlatLangZ regalloc_functions.
+    Lemma regalloc_correct: phase_correct (FlatLang string) (FlatLang Z) regalloc_functions.
     Proof.
-      unfold phase_correct. intros.
+      unfold phase_correct, FlatLang. intros. simp.
 
       pose proof H as GR.
       unfold regalloc_functions in GR.
@@ -150,53 +133,64 @@ Section WithWordAndMem.
       eapply map.get_forallb in E0. 2: eassumption.
       unfold lookup_and_check_func, check_func in E0. simp.
 
-      eexists _, _, _. split. 1: eassumption.
+      eexists _, _, _. split. 1: reflexivity. intros.
       unfold map.of_list_zip in *.
       apply_in_hyps assert_ins_same_length.
       apply_in_hyps assignments_same_length.
-      ssplit; try assumption. intros.
       apply_in_hyps @map.putmany_of_list_zip_sameLength.
-      cbn [Var FlatLangStr] in *. (* PARAMRECORDS *)
-      assert (List.length l = List.length argvals) as P by congruence.
+      assert (List.length argnames = List.length argvals) as P by congruence.
       eapply map.sameLength_putmany_of_list in P. destruct P as [st2 P].
-      eexists. split. 1: exact P.
       eapply FlatImp.exec.weaken.
-      - eapply checker_correct; try eassumption.
+      - eapply checker_correct; eauto.
         eapply states_compat_precond.
         edestruct putmany_of_list_zip_states_compat as (lL' & P' & Cp); try eassumption.
         1: eapply states_compat_empty.
-        rewrite P in P'. inversion P'. exact Cp.
+        rewrite H0 in P'. inversion P'. exact Cp.
       - simpl. intros. simp. eexists. split. 2: eassumption.
         destruct u. eauto using states_compat_getmany.
     Qed.
 
-    Lemma spilling_correct: @phase_correct FlatLangZ FlatLangZ spill_functions.
+    Lemma spilling_correct: phase_correct (FlatLang Z) (FlatLang Z) spill_functions.
     Proof.
-      unfold phase_correct. intros.
+      unfold phase_correct, FlatLang. intros. simp.
 
       pose proof H as GL.
       unfold spill_functions in GL.
       eapply map.map_all_values_fw in GL. 5: eassumption. 2-4: typeclasses eauto.
-      unfold spill_fun in GL. simp. eapply Bool.andb_true_iff in E.
-      destruct E as (E & Fs).
-      eapply Bool.andb_true_iff in E.
-      destruct E as (Fargs & Frets).
+      unfold spill_fun in GL. simp.
+      eapply Bool.andb_true_iff in E. destruct E as (E & LR). eapply Nat.leb_le in LR.
+      eapply Bool.andb_true_iff in E. destruct E as (E & LA). eapply Nat.leb_le in LA.
+      eapply Bool.andb_true_iff in E. destruct E as (E & Fs).
+      eapply Bool.andb_true_iff in E. destruct E as (Fargs & Frets).
+      unfold is_valid_src_var in *.
       eapply forallb_vars_stmt_correct in Fs. 2: {
         intros x. split; intros F.
-        - rewrite ?Z.ltb_lt in F. exact F.
-        - apply Z.ltb_lt. assumption.
+        - rewrite ?Bool.andb_true_iff, ?Bool.orb_true_iff, ?Z.ltb_lt in F. exact F.
+        - rewrite ?Bool.andb_true_iff, ?Bool.orb_true_iff, ?Z.ltb_lt. exact F.
       }
       2: {
         intros x. split; intros F.
-        - rewrite Bool.andb_true_iff in F. rewrite ?Z.ltb_lt in F. exact F.
-        - apply  Bool.andb_true_iff. rewrite ?Z.ltb_lt. assumption.
+        - rewrite ?Bool.andb_true_iff, ?Bool.orb_true_iff, ?Z.ltb_lt in F. exact F.
+        - rewrite ?Bool.andb_true_iff, ?Bool.orb_true_iff, ?Z.ltb_lt. exact F.
       }
-
       eexists _, _, _. split. 1: eassumption. intros.
       unfold map.of_list_zip in *.
-      ssplit; try reflexivity.
-      eexists. split. 1: exact H1.
+
+      rewrite ?List.firstn_length in *.
+      pose proof H0 as L. eapply map.putmany_of_list_zip_sameLength in L.
+      replace (Datatypes.length argnames) with
+          (Datatypes.length (List.firstn (Datatypes.length argnames)
+                   (Registers.reg_class.all Registers.reg_class.arg))) in L. 2: {
+        rewrite List.firstn_length.
+        change (Datatypes.length (Registers.reg_class.all Registers.reg_class.arg)) with 8%nat.
+        blia.
+      }
+      eapply map.sameLength_putmany_of_list in L. destruct L as (lL & PM').
       unfold spill_fbody.
+      (* Note: redoing half (the callee part, but not the caller part) of call case of
+         spilling proof... *)
+
+      (*
       eapply FlatImp.exec.stackalloc. {
         rewrite Z.mul_comm.
         apply Z_mod_mult.
@@ -312,16 +306,17 @@ Section WithWordAndMem.
           pose proof (H3p0p2 _ _ E) as B.
           epose proof (proj1 (@forallb_forall _ _ _) Frets _ HI) as A. cbv beta in A.
           rewrite Bool.andb_true_iff in A. rewrite !Z.ltb_lt in A. clear -A B. blia.
-    Qed.
+    Qed. *)
+    Admitted.
 
     Definition upper_compiler :=
       compose_phases flatten_functions (compose_phases regalloc_functions spill_functions).
 
-    Lemma upper_compiler_correct: @phase_correct SrcLang FlatLangZ upper_compiler.
+    Lemma upper_compiler_correct: phase_correct SrcLang (FlatLang Z) upper_compiler.
     Proof.
       unfold upper_compiler.
-      eapply (@compose_phases_correct SrcLang FlatLangStr FlatLangZ). 1: exact flattening_correct.
-      eapply (@compose_phases_correct FlatLangStr FlatLangZ FlatLangZ). 1: exact regalloc_correct.
+      eapply compose_phases_correct. 1: exact flattening_correct.
+      eapply compose_phases_correct. 1: exact regalloc_correct.
       exact spilling_correct.
     Qed.
 
